theories/interpreter_ctx.v
@@ -39,9 +39,15 @@ Definition reduce_ctx (hs hs': host_state) (cfg cfg': cfg_tuple_ctx) : Prop :=
 
 Ltac red_ctx_simpl :=
   repeat lazymatch goal with
-  | _: _ |- reduce _ _ _ (foldl closure_ctx_fill _ _) _ _ _ (foldl closure_ctx_fill _ _) =>
+  | |- reduce _ _ _ (((_, ?lcs) :: ?ccs) ⦃ _ ⦃ _ ⦄ ⦄) _ _ _ (((_, ?lcs) :: ?ccs) ⦃ _ ⦃ _ ⦄ ⦄) =>
+      apply reduce_focus_ctx_id
+  | |- reduce _ _ _ (((_, _) :: ?ccs) ⦃ _ ⦃ _ ⦄ ⦄) _ _ _ (((_, _) :: ?ccs) ⦃ _ ⦃ _ ⦄ ⦄) =>
+      apply reduce_focus_ctx
+  | |- reduce _ _ _ (?ccs ⦃ _ ⦃ _ ⦄ ⦄) _ _ _ (?ccs ⦃ _ ⦃ _ ⦄ ⦄) =>
       apply (list_closure_ctx_eval.(ctx_reduce))
-  | _: _ |- reduce _ _ _ (foldl label_ctx_fill _ _) _ _ _ (foldl label_ctx_fill _ _) =>
+  | |- reduce _ _ _ (foldl closure_ctx_fill _ _) _ _ _ (foldl closure_ctx_fill _ _) =>
+      apply (list_closure_ctx_eval.(ctx_reduce))
+  | |- reduce _ _ _ (foldl label_ctx_fill _ _) _ _ _ (foldl label_ctx_fill _ _) =>
       apply (list_label_ctx_eval.(ctx_reduce))
   end.
 
@@ -49,21 +55,35 @@ Ltac infer_hole :=
   repeat lazymatch goal with
   | |- context C [vs_to_es _] =>
       rewrite /vs_to_es
+  | |- ?l1 ++ ?l2 = ?x1 :: ?x2 :: ?x3 :: ?x4 :: ?l2 =>
+      try by instantiate (1 := [::x1; x2; x3; x4]) => //
+  | |- ?l1 ++ ?l2 = ?x1 :: ?x2 :: ?x3 :: ?l2 =>
+      try by instantiate (1 := [::x1; x2; x3]) => //
+  | |- ?l1 ++ ?l2 = ?x1 :: ?x2 :: ?l2 =>
+      try by instantiate (1 := [::x1; x2]) => //
+  | |- ?l1 ++ ?l2 = ?x :: ?l2 =>
+      try by instantiate (1 := [::x]) => //
+  | |- ?l ++ ?les = ?les =>
+      try by instantiate (1 := nil) => //
+  | |- ?l1 ++ ?l2 = ?l3 ++ ?x :: ?l2 =>
+      try instantiate (1 := l3 ++ [::x]); rewrite -catA => //
   | _: _ |- ?l ++ _ = ?l ++ _ =>
       f_equal => //
-  | _: _ |- ?l1 ++ ?l2 = ?x :: ?l2 =>
-      try instantiate (1 := [::x]) => //
-  | _: _ |- ?l1 ++ ?l2 = ?x1 :: ?x2 :: ?l2 =>
-      instantiate (1 := [::x1; x2]) => //
-  | _: _ |- ?l1 ++ ?l2 = ?l3 ++ ?x :: ?l2 =>
-      try instantiate (1 := l3 ++ [::x]); rewrite -catA => //
   | |- context C [ _ ++ [::] ] =>
       rewrite cats0
+  | |- context C [v_to_e_list (rev (?x :: ?l2))] =>
+      rewrite rev_cons -cats1 -v_to_e_cat => //
   | |- context C [v_to_e_list (rev (?l1 ++ ?l2))] =>
       rewrite rev_cat -v_to_e_cat => //
+  | |- context C [v_to_e_list [:: ?x] ] =>
+      unfold v_to_e_list, v_to_e => //=
   | |- context C [ ( _ ++ _) ++ _ ] =>
       rewrite -catA
   end.
+
+Ltac resolve_reduce_ctx vs es :=
+  (* Sometimes 1 infer_hole isn't enough, which supposedly shouldn't occur *)
+  unfold reduce_ctx; red_ctx_simpl => //=; try (eapply r_label with (lh := LH_base (rev vs) es) => /=; do 2 infer_hole => /=).
 
 Ltac resolve_valid_ccs :=
   repeat lazymatch goal with
@@ -75,7 +95,121 @@ Ltac resolve_valid_ccs :=
         apply/orP; (try by left); (try by right)
     end.
 
-Definition run_one_step_ctx (hs: host_state) (cfg: cfg_tuple_ctx) : valid_cfg_ctx cfg -> {hs' & {cfg' | reduce_ctx hs hs' cfg cfg' /\ valid_cfg_ctx cfg'}} + False.
+Ltac get_cc ccs Hvalid :=
+  let fc := fresh "fc" in 
+  let lcs := fresh "lcs" in 
+  let ccs' := fresh "ccs'" in 
+  destruct ccs as [ | [fc lcs] ccs']; first by unfold valid_cfg_ctx, valid_ccs in Hvalid; inversion Hvalid.
+
+Definition s_of_cfg (cfg: cfg_tuple_ctx) :=
+  match cfg with
+  | (s, _, _, _) => s
+  end.
+
+Definition es_of_cfg (cfg: cfg_tuple_ctx) :=
+  match cfg with
+  | (_, ccs, sc, oe) => ccs ⦃ sc ⦃ olist oe ⦄ ⦄
+  end.
+
+Inductive run_step_ctx_result (hs: host_state) (cfg: cfg_tuple_ctx): Type :=
+| RSC_normal hs' cfg':
+  reduce_ctx hs hs' cfg cfg' ->
+  run_step_ctx_result hs cfg
+| RSC_value:
+  const_list (es_of_cfg cfg) ->
+  run_step_ctx_result hs cfg
+| RSC_error:
+  forall ts, (config_typing (s_of_cfg cfg) empty_frame (es_of_cfg cfg) ts -> False) ->
+  run_step_ctx_result hs cfg
+| RSC_admit:
+  False ->
+  run_step_ctx_result hs cfg
+.
+
+Definition rsc_admit_inhab : False.
+Admitted.
+
+
+Ltac admit_rsc :=
+  by apply RSC_admit; apply rsc_admit_inhab.
+
+
+Notation "<< hs , cfg >>" := (@RSC_normal _ _ hs cfg).
+
+Definition empty_label_ctx := Build_label_ctx nil 0 nil nil.
+
+Lemma nth_nth_error {T: Type}: forall (l: list T) k x0 v,
+    List.nth_error l k = Some v ->
+    nth x0 l k = v.
+Proof.
+  elim; first by case => //.
+  move => ???; case => //=.
+  by move => ?? [<-].
+Qed.
+
+Definition run_ctx_br: forall hs s ccs sc j,
+  valid_cfg_ctx (s, ccs, sc, Some (AI_basic (BI_br j))) ->
+  run_step_ctx_result hs (s, ccs, sc, Some (AI_basic (BI_br j))).
+Proof.
+  intros hs s ccs [vs es] j Hvalid.
+  get_cc ccs Hvalid.
+  destruct (j < length lcs) eqn:Hlablen.
+  - destruct (List.nth_error lcs j) as [lab | ] eqn:Htar; last by apply List.nth_error_None in Htar; move/ltP in Hlablen; lias.
+    destruct lab as [lvs lk lces les].
+    destruct (lk <= length vs) eqn:Hvslen.
+    + apply <<hs, (s, ((fc, drop (S j) lcs) :: ccs'), (take lk vs ++ lvs, lces ++ les), None)>>.
+      apply reduce_focus_ctx => //=.
+      rewrite - (cat_take_drop (j.+1) lcs) drop_size_cat; last by rewrite size_takel => //.
+      rewrite foldl_cat.
+      apply list_label_ctx_eval.(ctx_reduce) => //=.
+      rewrite /fmask0.
+      rewrite (take_nth empty_label_ctx) => //.
+      rewrite foldl_rcons.
+      apply nth_nth_error with (x0 := empty_label_ctx) in Htar.
+      rewrite Htar => /=.
+      rewrite - (cat_take_drop lk vs) take_size_cat; last by rewrite size_takel => //.
+      rewrite /vs_to_es rev_cat -v_to_e_cat rev_cat -v_to_e_cat -cat1s -catA.
+      resolve_reduce_ctx lvs les; last rewrite catA; eauto => //=.
+      simpl.
+      apply r_simple; eapply rs_br.
+      { by apply v_to_e_const. }
+      { by rewrite v_to_e_length length_is_size size_rev size_takel. }
+      { apply lh_ctx_fill_aux with (acc := (LH_base (rev (drop lk vs)) es)) (lcs := take j lcs) => /=.
+        rewrite ctx_to_lh_aux_len => /=.
+        repeat rewrite - catA => /=.
+        rewrite add0n length_is_size size_takel; rewrite length_is_size in Hlablen; by lias => //=.
+      }
+      
+    + (* Not enough values *)
+      by admit_rsc.
+  - (* Not enough labels *)
+    by admit_rsc.
+Qed.
+    
+Definition run_ctx_return: forall hs s ccs sc,
+  valid_cfg_ctx (s, ccs, sc, Some (AI_basic BI_return)) ->
+  run_step_ctx_result hs (s, ccs, sc, Some (AI_basic BI_return)).
+Proof.  
+  intros hs s ccs [vs es] Hvalid.
+  get_cc ccs Hvalid.
+  destruct fc as [lvs lk lf les].
+  destruct (lk <= length vs) eqn:Hvslen.
+  - apply <<hs, (s, ccs', (take lk vs ++ lvs, les), None)>> => /=.
+    rewrite - (cat_take_drop lk vs) take_size_cat; last by rewrite size_takel => //.
+    rewrite /vs_to_es rev_cat -v_to_e_cat rev_cat -v_to_e_cat -cat1s -catA.
+    resolve_reduce_ctx lvs les; last rewrite catA; eauto => //=.
+    apply r_simple; eapply rs_return.
+    { by apply v_to_e_const. }
+    { by rewrite v_to_e_length length_is_size size_rev size_takel. }
+    { apply lh_ctx_fill_aux with (acc := (LH_base (rev (drop lk vs)) es)) (lcs := lcs) => /=.
+      by repeat rewrite - catA => /=.
+    }
+  - (* Not enough values *)
+    by admit_rsc.
+Qed.
+    
+(* One step of execution; does not perform the context update in the end to shift to the new instruction. *)
+Definition run_one_step_ctx (hs: host_state) (cfg: cfg_tuple_ctx) : valid_cfg_ctx cfg -> run_step_ctx_result hs cfg.
 Proof.
   move => Hvalid.
   destruct cfg as [[[s ccs] sc] oe].
@@ -86,7 +220,8 @@ Proof.
     destruct Hvalid as [? Heq]; move/eqP in Heq; subst es.
     destruct ccs as [ | [fc lcs] ccs'].
     { (* entire instruction is const *)
-      right. admit.
+      apply RSC_value => /=.
+      by rewrite cats0; apply v_to_e_const.
     }
     { destruct lcs as [ | lc lcs'].
       (* Exitting a local *)
@@ -96,59 +231,37 @@ Proof.
         {
           destruct les as [ | e les'].
           { (* No instruction in the hole *)
-            left; exists hs, (s, ccs', (vs ++ lvs, nil), None) => /=.
-            split; last by resolve_valid_ccs.
-            red_ctx_simpl => //.
-            repeat rewrite cats0.
-            eapply r_label with (lh := LH_base (rev lvs) nil) => /=; infer_hole.
+            apply <<hs, (s, ccs', (vs ++ lvs, nil), None)>> => /=.
+            resolve_reduce_ctx lvs (nil: list administrative_instruction).
             by apply r_simple, rs_local_const; [ by apply v_to_e_const | by rewrite length_is_size v_to_e_size size_rev ].
           }
-          { (* e is in the hole; push any context e has into the stack *)
-            remember (ctx_update ccs' (vs ++ lvs, les') e) as cfg_new; symmetry in Heqcfg_new.
+          { (* e is in the hole *)
+          (*  remember (ctx_update ccs' (vs ++ lvs, les') e) as cfg_new; symmetry in Heqcfg_new.
             destruct cfg_new as [[[ccs0 [vs0 es0]] oe] | ].
-            - destruct (valid_ccs ccs0 oe) eqn:Hccsnil.
-              { left; exists hs, (s, ccs0, (vs0, es0), oe).
-                split.
-                + apply ctx_update_fill in Heqcfg_new.
-                  unfold reduce_ctx.
-                  rewrite -Heqcfg_new => /=.
-                  red_ctx_simpl => //.
-                  rewrite cats0.
-                  eapply r_label with (lh := LH_base (rev lvs) (e :: les')) => /=; infer_hole.
-                  by apply r_simple, rs_local_const; [ by apply v_to_e_const | by rewrite length_is_size v_to_e_size size_rev ].
-                + split => //; by apply ctx_update_valid in Heqcfg_new.
-              }
-              { (* The generated context is invalid as there are no wrapping contexts left*)
-                right. admit.
-              }
-            - (* Same -- invalid context *)
-              right. admit.
+            - destruct (valid_ccs ccs0 oe) eqn:Hccsnil. *)
+            apply <<hs, (s, ccs', (vs ++ lvs, les'), Some e)>> => /=.
+            resolve_reduce_ctx lvs (e :: les').
+            by apply r_simple, rs_local_const; [ by apply v_to_e_const | by rewrite length_is_size v_to_e_size size_rev ].
           }
         }
-        (* length doesn't match -- no reduce *)
-        { right. admit. }
+        (* length doesn't match -- ill-typed *)
+        { by admit_rsc. }
       }
       (* Exitting a label *)
       { destruct lc as [lvs lk lces les].
         destruct les as [ | e les'].
         { (* No instruction in the hole still *)
-          left; exists hs, (s, (fc, lcs') :: ccs', (vs ++ lvs, nil), None) => /=.
-          split => //.
-          red_ctx_simpl => //.
-          repeat rewrite cats0.
-          eapply r_label with (lh := LH_base (rev (FC_val fc)) (FC_post fc)) => /=; infer_hole.
-          apply r_local => /=.
+          apply <<hs, (s, (fc, lcs') :: ccs', (vs ++ lvs, nil), None)>> => /=.
+          resolve_reduce_ctx (FC_val fc) (FC_post fc).
+          eapply r_local.
           red_ctx_simpl => //=.
           unfold fmask0, label_ctx_fill => /=.
-          eapply r_label with (lh := LH_base (rev lvs) nil) => /=; infer_hole.
+          eapply r_label with (lh := LH_base (rev lvs) nil) => /=; infer_hole; eauto => /=.
           apply r_simple, rs_label_const; by apply v_to_e_const.
         }
         { (* e is in the hole *)
-          left; exists hs, (s, (fc, lcs') :: ccs', (vs ++ lvs, ), None) => /=.
-          split => //.
-          red_ctx_simpl => //.
-          rewrite cats0.
-          eapply r_label with (lh := LH_base (rev (FC_val fc)) (FC_post fc)) => /=; infer_hole.
+          apply <<hs, (s, (fc, lcs') :: ccs', (vs ++ lvs, les'), Some e)>> => /=.
+          resolve_reduce_ctx (FC_val fc) (FC_post fc).
           apply r_local => /=.
           red_ctx_simpl => //=.
           unfold fmask0, label_ctx_fill => /=.
@@ -156,7 +269,9 @@ Proof.
           apply r_simple, rs_label_const; by apply v_to_e_const.
         }
       }
+    }
   }
+  (* Execute an instruction *)
   { destruct e as [
       (* AI_basic *) [
       (* BI_unreachable *) |
@@ -177,67 +292,108 @@ Proof.
       (* BI_tee_local j *) j |
       (* BI_get_global j *) j |
       (* BI_set_global j *) j |
-      (* BI_load t [Some (tp, sx)|None] a off *) t [[tp sx]|] a off |
-      (* BI_store t [Some tp|None] a off *) t [tp|] a off |
+      (* BI_load t [Some (tp, sx)|None] a off *) t ops(*[[tp sx]|]*) a off |
+      (* BI_store t [Some tp|None] a off *) t op(*[tp|]*) a off |
       (* BI_current_memory *) |
       (* BI_grow_memory *) |
       (* BI_const _ *) |
       (* BI_unop t op *) t op |
       (* BI_binop t op *) t op |
-      (* BI_testop [T_i32|T_i64|T_f32|T_f64] testop *) [| | |] testop |
+      (* BI_testop [T_i32|T_i64|T_f32|T_f64] testop *) t(*[| | |]*) testop |
       (* BI_relop t op *) t op |
-      (* BI_cvtop t2 [CVO_convert|CVO_reinterpret] t1 sx *) t2 [|] t1 sx ] |
+      (* BI_cvtop t2 [CVO_convert|CVO_reinterpret] t1 sx *) t2 cvtop (*[|]*) t1 sx ] |
       (* AI_trap *) |
       (* AI_invoke a *) a |
       (* AI_label ln les es *) ln les es |
-      (* AI_local ln lf es *) ln lf es ].
+      (* AI_local ln lf es *) ln lf es ]; destruct sc as [vs0 es0].
 
-    * (* AI_basic BI_unreachable *)
-      apply <<hs, s, f, vs_to_es ves ++ [:: AI_trap]>>'.
-      by apply reduce_unreachable.
+    - (* AI_basic BI_unreachable *)
+      apply <<hs, (s, ccs, (vs0, es0), Some AI_trap)>> => /=.
+      resolve_reduce_ctx vs0 es0.
+      by apply r_simple, rs_unreachable.
 
-    * (* AI_basic BI_nop *)
-      apply <<hs, s, f, vs_to_es ves>>'.
-      by apply reduce_nop.
+    - (* AI_basic BI_nop *)
+      apply <<hs, (s, ccs, (vs0, es0), None)>> => /=.
+      resolve_reduce_ctx vs0 es0.
+      by apply r_simple, rs_nop.
 
-    * (* AI_basic BI_drop *)
-      destruct ves as [|v ves'] eqn:Heqves.
+    - (* AI_basic BI_drop *)
+      destruct vs0 as [ | v vs0].
       + (* [::] *)
-        apply RS''_error. by apply drop_error.
-      + (* v :: ves' *)
-        apply <<hs, s, f, vs_to_es ves'>>'. by apply reduce_drop.
-
-    * (* AI_basic BI_select *)
-      destruct ves as [|v3 [|v2 [|v1 ves']]];
-        try by (apply RS''_error; apply select_error_size).
-      (* [:: v3, v2, v1 & ves'] *)
-      destruct v3 as [c| | |] eqn:?;
-        try by
-          (apply RS''_error; eapply select_error_i32 with (v3 := v3); subst v3).
+        by admit_rsc.
+      + (* v :: vs0 *)
+        apply <<hs, (s, ccs, (vs0, es0), None)>> => /=.
+        resolve_reduce_ctx vs0 es0.
+        by apply r_simple, rs_drop.
+      
+    - (* AI_basic BI_select *)
+      destruct vs0 as [|v3 [|v2 [|v1 vs0]]].
+        (*  try by (apply RS''_error; apply select_error_size). *)
+        1,2,3: by admit_rsc.
+      (* [:: v3, v2, v1 & vs0] *)
+        destruct v3 as [c| | |] eqn:?.
+        2,3,4: by admit_rsc.
+ (*       try by
+          (apply RS''_error; eapply select_error_i32 with (v3 := v3); subst v3).*)
       (* VAL_int32 c *)
-      destruct (c == Wasm_int.int_zero i32m) eqn:?.
+      destruct (c == Wasm_int.int_zero i32m) eqn:Heq0; move/eqP in Heq0.
       + (* true *)
-        apply <<hs, s, f, vs_to_es (v2 :: ves')>>'.
-        by apply reduce_select_false.
+        apply <<hs, (s, ccs, (vs0, es0), Some (AI_basic (BI_const v2)))>> => /=.
+        resolve_reduce_ctx vs0 es0.
+        by apply r_simple; apply rs_select_false.
       + (* false *)
-        apply <<hs, s, f, vs_to_es (v1 :: ves')>>'.
-        by apply reduce_select_true; clear run_step_aux; lias.
+        apply <<hs, (s, ccs, (vs0, es0), Some (AI_basic (BI_const v1)))>> => /=.
+        resolve_reduce_ctx vs0 es0.
+        by apply r_simple; apply rs_select_true.
 
-    * (* AI_basic (BI_block (Tf t1s t2s) es) *)
-      destruct (length ves >= length t1s) eqn:?.
+    - (* AI_basic (BI_block (Tf t1s t2s) es) *)
+      destruct (length vs0 >= length t1s) eqn:Hlen.
       + (* true *)
-        destruct (split_n ves (length t1s)) as [ves' ves''] eqn:?.
+        destruct (split_n vs0 (length t1s)) as [ves' ves''] eqn:Hsplit.
         remember (AI_label (length t2s) [::] (vs_to_es ves' ++ to_e_list es)) as e'.
-        apply <<hs, s, f, vs_to_es ves'' ++ [:: e']>>'.
-        by subst e'; eapply reduce_block.
+        apply <<hs, (s, ccs, (ves'', es0), Some e')>> => /=.
+        red_ctx_simpl => //.
+        rewrite split_n_is_take_drop in Hsplit; injection Hsplit as ??; subst.
+        eapply r_label with (lh := LH_base (rev (drop (length t1s) vs0)) es0) => /=; infer_hole => /=.
+        2: { instantiate (1 := (v_to_e_list (rev (take (length t1s) vs0))) ++ [::AI_basic (BI_block (Tf t1s t2s) es)]).
+             repeat rewrite catA.
+             rewrite v_to_e_cat -rev_cat cat_take_drop.
+             by infer_hole.
+        }
+        apply r_simple; eapply rs_block; eauto; first by apply v_to_e_const.
+        rewrite v_to_e_length.
+        repeat rewrite length_is_size.
+        repeat rewrite length_is_size in Hlen.
+        by rewrite size_rev size_takel.
       + (* false *)
-        apply RS''_error.
+        by admit_rsc.
+        (* apply RS''_error.
         (* TODO should use length in lemmas instead? *)
         repeat rewrite length_is_size in Heqb.
-        by apply block_error; clear - Heqb; lias.
+        by apply block_error; clear - Heqb; lias.*)
 
-    * (* AI_basic (BI_loop (Tf t1s t2s) es) *)
-      destruct (length ves >= length t1s) eqn:?.
+    - (* AI_basic (BI_loop (Tf t1s t2s) es) *)
+      destruct (length vs0 >= length t1s) eqn:Hlen.
+      + (* true *)
+        destruct (split_n vs0 (length t1s)) as [ves' ves''] eqn:Hsplit.
+        remember (AI_label (length t1s) [::AI_basic (BI_loop (Tf t1s t2s) es)] (vs_to_es ves' ++ to_e_list es)) as e'.
+        apply <<hs, (s, ccs, (ves'', es0), Some e')>> => /=.
+        red_ctx_simpl => //.
+        rewrite split_n_is_take_drop in Hsplit; injection Hsplit as ??; subst.
+        eapply r_label with (lh := LH_base (rev (drop (length t1s) vs0)) es0) => /=; infer_hole => /=.
+        2: { instantiate (1 := (v_to_e_list (rev (take (length t1s) vs0))) ++ [::AI_basic (BI_loop (Tf t1s t2s) es)]).
+             repeat rewrite catA.
+             rewrite v_to_e_cat -rev_cat cat_take_drop.
+             by infer_hole.
+        }
+        apply r_simple; eapply rs_loop; eauto; first by apply v_to_e_const.
+        rewrite v_to_e_length.
+        repeat rewrite length_is_size.
+        repeat rewrite length_is_size in Hlen.
+        by rewrite size_rev size_takel.
+      + (* false *)
+        by admit_rsc.
+      (*destruct (length ves >= length t1s) eqn:?.
       + (* true *)
         destruct (split_n ves (length t1s)) as [ves' ves''] eqn:?.
         apply <<hs, s, f, vs_to_es ves''
@@ -246,177 +402,236 @@ Proof.
         by apply reduce_loop.
       + (* false *)
         apply RS''_error.
-        apply loop_error; repeat rewrite -length_is_size; clear run_step_aux; lias.
-
-    * (* AI_basic (BI_if tf es1 es2) *)
-      destruct ves as [|v ves'] eqn:?;
-        try by (apply RS''_error; apply if_error_0).
+        apply loop_error; repeat rewrite -length_is_size; clear run_step_aux; lias.*)
+        
+    - (* AI_basic (BI_if tf es1 es2) *)
+      destruct vs0 as [|v vs0]; first by admit_rsc.
+ (*       try by (apply RS''_error; apply if_error_0). *)
       (* v :: ves' *)
-      destruct v as [c| | |] eqn:?;
-        try by (apply RS''_error; eapply if_error_typeof => //).
+      destruct v as [c| | |].
+      2,3,4: by admit_rsc. 
       (* VAL_int32 c *)
-      destruct (c == Wasm_int.int_zero i32m) eqn:?.
+      destruct (c == Wasm_int.int_zero i32m) eqn:Heq0; move/eqP in Heq0.
       + (* true *)
-        apply <<hs, s, f, vs_to_es ves' ++ [:: AI_basic (BI_block tf es2)]>>'.
-        by eapply reduce_if_false.
+        apply <<hs, (s, ccs, (vs0, es0), Some (AI_basic (BI_block tf es2)))>> => /=.
+        resolve_reduce_ctx vs0 es0.
+        by apply r_simple; apply rs_if_false.
       + (* false *)
-        apply <<hs, s, f, vs_to_es ves' ++ [:: AI_basic (BI_block tf es1)]>>'.
-        by eapply reduce_if_true.
+        apply <<hs, (s, ccs, (vs0, es0), Some (AI_basic (BI_block tf es1)))>> => /=.
+        resolve_reduce_ctx vs0 es0.
+        by apply r_simple; apply rs_if_true.
 
-    * (* AI_basic (BI_br j) *)
-      apply break(j, ves).
-      by apply break_br.
+    - (* AI_basic (BI_br j) *)
+      by apply run_ctx_br.
 
-    * (* AI_basic (BI_br_if j) *)
-      destruct ves as [|v ves'];
-        try by (apply RS''_error; apply br_if_error_0).
+    - (* AI_basic (BI_br_if j) *)
+      destruct vs0 as [|v vs0]; first by admit_rsc.
+     (*   try by (apply RS''_error; apply br_if_error_0). *)
       (* v :: ves' *)
-      destruct v as [c| | |] eqn:?;
-        try by (apply RS''_error; eapply br_if_error_i32 with (v := v); subst v).
+      destruct v as [c| | |] eqn:?.
+      2,3,4: by admit_rsc.
+      (*  try by (apply RS''_error; eapply br_if_error_i32 with (v := v); subst v). *)
       (* VAL_int32 c *)
-      destruct (c == Wasm_int.int_zero i32m) eqn:?.
-      ** (* true *)
-         apply <<hs, s, f, vs_to_es ves'>>'.
-         by eapply reduce_br_if_false.
-      ** (* false *)
-         apply <<hs, s, f, vs_to_es ves' ++ [:: AI_basic (BI_br j)]>>'.
-         by eapply reduce_br_if_true; clear run_step_aux; lias.
+      destruct (c == Wasm_int.int_zero i32m) eqn:Heqc; move/eqP in Heqc.
+      + (* 0 *)
+        apply <<hs, (s, ccs, (vs0, es0), None)>> => /=.
+        resolve_reduce_ctx vs0 es0.
+        by apply r_simple; apply rs_br_if_false.
+      + (* not 0 *)
+        apply <<hs, (s, ccs, (vs0, es0), Some (AI_basic (BI_br j)))>> => /=.
+        resolve_reduce_ctx vs0 es0.
+        by apply r_simple; apply rs_br_if_true.
 
-    * (* AI_basic (BI_br_table js j) *)
-      destruct ves as [|v ves'];
-        try by (apply RS''_error; apply br_table_error_0).
+    - (* AI_basic (BI_br_table js j) *)
+      destruct vs0 as [|v vs0]; first by admit_rsc.
+       (* try by (apply RS''_error; apply br_table_error_0).*)
       (* v :: ves' *)
-      destruct v as [c| | |] eqn:?;
-        try by (apply RS''_error; eapply br_table_error_i32 with (v := v); subst v).
+      destruct v as [c| | |] eqn:?.
+      2,3,4: by admit_rsc.
+      (*  try by (apply RS''_error; eapply br_table_error_i32 with (v := v); subst v). *)
       remember (Wasm_int.nat_of_uint i32m c) as k.
-      destruct (k < length js) eqn:?.
+      destruct (k < length js) eqn:Hlen.
       + (* true *)
-        destruct (List.nth_error js k) as [js_at_k|] eqn:?.
-        -- (* Some js_at_k *)
-           apply <<hs, s, f, vs_to_es ves' ++ [::AI_basic (BI_br js_at_k)]>>'.
-           by apply reduce_br_table with (k := k).
-        -- (* None *)
-           apply RS''_error.
-           by apply br_table_error_kth with (k := k) (c := c) (ves' := ves').
+        destruct (List.nth_error js k) as [js_at_k|] eqn: Hnth.
+        * (* Some js_at_k *)
+          apply <<hs, (s, ccs, (vs0, es0), Some (AI_basic (BI_br js_at_k)))>> => /=.
+          resolve_reduce_ctx vs0 es0.
+          by apply r_simple; subst; apply rs_br_table.
+        * (* None *)
+          by admit_rsc.
+          (* apply RS''_error.
+           by apply br_table_error_kth with (k := k) (c := c) (ves' := ves'). *)
       + (* false *)
-        apply <<hs, s, f, vs_to_es ves' ++ [::AI_basic (BI_br j)]>>'.
-        by apply reduce_br_table_length with (k := k); clear run_step_aux; lias.
+        apply <<hs, (s, ccs, (vs0, es0), Some (AI_basic (BI_br j)))>> => /=.
+        resolve_reduce_ctx vs0 es0.
+        by apply r_simple; subst; apply rs_br_table_length; lias.
+        
+    - (* AI_basic BI_return *)
+      by apply run_ctx_return.
 
-    * (* AI_basic BI_return *)
-      apply RS''_return with (rvs := ves).
-      by left => //.
-
-    * (* AI_basic (BI_call j) *)
-      destruct (List.nth_error f.(f_inst).(inst_funcs) j) as [a|] eqn:?.
+    - (* AI_basic (BI_call j) *)
+      get_cc ccs Hvalid.
+      destruct (List.nth_error fc.(FC_frame).(f_inst).(inst_funcs) j) as [a|] eqn: Hnth.
       + (* Some a *)
-        apply <<hs, s, f, vs_to_es ves ++ [:: AI_invoke a]>>'.
-        by apply reduce_call.
+        apply <<hs, (s, (fc, lcs) :: ccs', (vs0, es0), Some (AI_invoke a))>>.
+        resolve_reduce_ctx vs0 es0.
+        by apply r_call.
       + (* None *)
-        apply RS''_error.
-        by apply call_error.
+        by admit_rsc.
+        (* apply RS''_error.
+        by apply call_error. *)
 
-    * (* AI_basic (BI_call_indirect j) *)
-      destruct ves as [|v ves'] eqn:?;
-        try by (apply RS''_error; apply call_indirect_error_0).
+    - (* AI_basic (BI_call_indirect j) *)
+      get_cc ccs Hvalid.    
+      destruct vs0 as [|v vs0]; first by admit_rsc.
+      (*  try by (apply RS''_error; apply call_indirect_error_0). *)
       (* v :: ves' *)
-      destruct v as [c| | |] eqn:?;
-        try by (apply RS''_error; eapply call_indirect_error_typeof => //).
+      destruct v as [c| | |] eqn:?.
+      2,3,4: by admit_rsc.
+       (* try by (apply RS''_error; eapply call_indirect_error_typeof => //). *)
       (* VAL_int32 c *)
+      remember (fc.(FC_frame)) as f.
       destruct (stab_addr s f (Wasm_int.nat_of_uint i32m c)) as [a|] eqn:?.
       + (* Some a *)
         destruct (List.nth_error s.(s_funcs) a) as [cl|] eqn:?.
-        -- (* Some cl *)
-           destruct (stypes s f.(f_inst) j == Some (cl_type cl)) eqn:?.
-           ** (* true *)
-              apply <<hs, s, f, vs_to_es ves' ++ [:: AI_invoke a]>>'.
-              by eapply reduce_call_indirect_success with (cl := cl).
-           ** (* false *)
-              apply <<hs, s, f, vs_to_es ves' ++ [:: AI_trap]>>'.
-              by eapply reduce_call_indirect_failure_1 with (cl := cl) (a := a).
-        -- (* None *)
+        * (* Some cl *)
+           destruct (stypes s f.(f_inst) j == Some (cl_type cl)) eqn:Hcl; move/eqP in Hcl.
+           -- (* true *)
+             apply <<hs, (s, (fc, lcs) :: ccs', (vs0, es0), Some (AI_invoke a))>>.
+             resolve_reduce_ctx vs0 es0.
+             by eapply r_call_indirect_success; subst; eauto.
+           -- (* false *)
+             apply <<hs, (s, (fc, lcs) :: ccs', (vs0, es0), Some (AI_trap))>>.
+             resolve_reduce_ctx vs0 es0.
+             by eapply r_call_indirect_failure1; subst; eauto.
+              (*apply <<hs, s, f, vs_to_es ves' ++ [:: AI_trap]>>'.
+              by eapply reduce_call_indirect_failure_1 with (cl := cl) (a := a).*)
+        * (* None *)
+          by admit_rsc.
+          (*
            apply RS''_error.
-           by eapply call_indirect_error_ath with (a := a).
+           by eapply call_indirect_error_ath with (a := a). *)
       + (* None *)
-        apply <<hs, s, f, vs_to_es ves' ++ [:: AI_trap]>>'.
-        by eapply reduce_call_indirect_failure_2.
+        apply <<hs, (s, (fc, lcs) :: ccs', (vs0, es0), Some (AI_trap))>>.
+        resolve_reduce_ctx vs0 es0.
+        by eapply r_call_indirect_failure2; subst.
 
-    * (* AI_basic (BI_get_local j) *)
+    - (* AI_basic (BI_get_local j) *)
+      get_cc ccs Hvalid.    
+      remember (fc.(FC_frame)) as f.
       destruct (j < length f.(f_locs)) eqn:?.
       + (* true *)
         destruct (List.nth_error f.(f_locs) j) as [vs_at_j|] eqn:?.
-        -- (* Some vs_at_j *)
-           apply <<hs, s, f, vs_to_es (vs_at_j :: ves)>>'.
-           by apply reduce_get_local.
-        -- (* None *)
-           apply RS''_error. by apply get_local_error_jth_none.
+        * (* Some vs_at_j *)
+          apply <<hs, (s, (fc, lcs) :: ccs', (vs_at_j :: vs0, es0), None)>>.
+          resolve_reduce_ctx vs0 es0.
+          by eapply r_get_local; subst.
+        * (* None *)
+          by admit_rsc.
+           (* apply RS''_error. by apply get_local_error_jth_none. *)
       + (* false *)
-        apply RS''_error. by apply get_local_error_length; clear run_step_aux; lias.
+        by admit_rsc.
+        (* apply RS''_error. by apply get_local_error_length; clear run_step_aux; lias. *)
 
-    * (* AI_basic (BI_set_local j) *)
-      destruct ves as [|v ves'] eqn:?.
+    - (* AI_basic (BI_set_local j) *)
+      get_cc ccs Hvalid.    
+      remember (fc.(FC_frame)) as f.
+      destruct vs0 as [|v vs0].
       + (* [::] *)
-        apply RS''_error. by apply set_local_error_0.
+        by admit_rsc.
+        (*apply RS''_error. by apply set_local_error_0.*)
       + (* v :: ves' *)
-        destruct (j < length f.(f_locs)) eqn:?.
-        -- (* true *)
-           apply <<hs, s, Build_frame (set_nth v f.(f_locs) j v) f.(f_inst), vs_to_es ves'>>'.
-           by eapply reduce_set_local.
-        -- (* false *)
-           apply RS''_error. by eapply set_local_error_length.
+        destruct (j < length f.(f_locs)) eqn:Hlen.
+        * (* true *)
+           apply <<hs, (s, ((Build_frame_ctx (fc.(FC_val)) fc.(FC_arity) (Build_frame (set_nth v f.(f_locs) j v) f.(f_inst)) fc.(FC_post)), lcs) :: ccs', (vs0, es0), None)>>.
+           resolve_reduce_ctx vs0 es0.
+           by eapply r_set_local; subst => //.
+        * (* false *)
+          by admit_rsc.
+           (*apply RS''_error. by eapply set_local_error_length.*)
 
-    * (* AI_basic (BI_tee_local j) *)
-      destruct ves as [|v ves'] eqn:?.
+    - (* AI_basic (BI_tee_local j) *)
+      destruct vs0 as [|v vs0].
       + (* [::] *)
-        apply RS''_error. by apply tee_local_error_0.
+        by admit_rsc.
+        (*apply RS''_error. by apply tee_local_error_0.*)
       + (* v :: ves' *)
-        apply <<hs, s, f, vs_to_es (v :: v :: ves') ++ [:: AI_basic (BI_set_local j)]>>'.
-        by eapply reduce_tee_local.
+        apply <<hs, (s, ccs, (v :: v :: vs0, es0), Some (AI_basic (BI_set_local j)))>> => /=.
+        resolve_reduce_ctx vs0 es0.
+        by eapply r_simple, rs_tee_local.
 
-    * (* AI_basic (BI_get_global j) *)
-      destruct (sglob_val s f.(f_inst) j) as [xx|] eqn:?.
+    - (* AI_basic (BI_get_global j) *)
+      get_cc ccs Hvalid.    
+      remember (fc.(FC_frame)) as f.
+      destruct (sglob_val s f.(f_inst) j) as [v|] eqn:Hsglob.
       + (* Some xx *)
-        apply <<hs, s, f, vs_to_es (xx :: ves)>>'.
-        by apply reduce_get_global.
+        apply <<hs, (s, (fc, lcs) :: ccs', (v :: vs0, es0), None)>>.
+        resolve_reduce_ctx vs0 es0.
+        by eapply r_get_global; subst.
       + (* None *)
-        apply RS''_error. by apply get_global_error.
+        by admit_rsc.
+        (* apply RS''_error. by apply get_global_error. *)
 
-    * (* AI_basic (BI_set_global j) *)
-      destruct ves as [|v ves'] eqn:?.
+    - (* AI_basic (BI_set_global j) *)
+      get_cc ccs Hvalid.    
+      remember (fc.(FC_frame)) as f.
+      destruct vs0 as [|v vs0].
       + (* [::] *)
-        apply RS''_error. by apply set_global_error_0.
+        by admit_rsc.
       + (* v :: ves' *)
-        destruct (supdate_glob s f.(f_inst) j v) as [s'|] eqn:?.
-        -- (* Some s' *)
-           apply <<hs, s', f, vs_to_es ves'>>'.
-           by eapply reduce_set_global => //.
-        -- (* None *)
-           apply RS''_error. by eapply set_global_error_jth.
+        destruct (supdate_glob s f.(f_inst) j v) as [s'|] eqn:Hsupdate.
+        * (* Some s' *)
+          apply <<hs, (s', (fc, lcs) :: ccs', (vs0, es0), None)>>.
+          resolve_reduce_ctx vs0 es0.
+          by eapply r_set_global; subst.
+        * (* None *)
+          by admit_rsc.
 
-    * (* AI_basic (BI_load t (Some (tp, sx)) a off) *)
-      (* TODO can this and the next branch be deduped? *)
-      destruct ves as [|v ves'] eqn:?.
+    - (* AI_basic (BI_load t ops (Some (tp, sx)) a off) *)
+      get_cc ccs Hvalid.    
+      remember (fc.(FC_frame)) as f.
+      destruct vs0 as [|v vs0].
       + (* [::] *)
-        apply RS''_error. by apply load_error_0.
+        by admit_rsc.
       + (* v :: ves' *)
-        destruct v as [c| | |] eqn:?;
-          try by (apply RS''_error; eapply load_error_typeof => //).
+        destruct v as [c| | |] eqn:?.
+        2,3,4: by admit_rsc.
         (* VAL_int32 c *)
         destruct (smem_ind s f.(f_inst)) as [j|] eqn:?.
-        -- (* Some j *)
+        * (* Some j *)
            destruct (List.nth_error s.(s_mems) j) as [mem_s_j|] eqn:?.
-           ** (* Some mem_s_j*)
-              destruct (load_packed sx (mem_s_j) (Wasm_int.N_of_uint i32m c) off (tp_length tp) (t_length t)) as [bs|] eqn:?.
-              ++ (* Some bs *)
-                 apply <<hs, s, f, vs_to_es (wasm_deserialise bs t :: ves')>>'.
-                 by apply reduce_load_packed_success with (mem_s_j := mem_s_j) (j := j) (c := c).
-              ++ (* None *)
-                 apply <<hs, s, f, vs_to_es ves' ++ [:: AI_trap]>>'.
-                 by apply reduce_load_packed_failure with (mem_s_j := mem_s_j) (j := j) (c := c).
-           ** (* None*)
-              apply RS''_error. by eapply load_error_jth with (j := j).
-        -- (* None *)
-           apply RS''_error. by eapply load_error_smem_ind.
+           { (* Some mem_s_j*)
+             destruct ops as [[tp sx] | ].
+             (* Some (tp, sx) *)
+             - destruct (load_packed sx (mem_s_j) (Wasm_int.N_of_uint i32m c) off (tp_length tp) (t_length t)) as [bs|] eqn:Hload.
+               + (* Some bs *)
+                 apply <<hs, (s, (fc, lcs) :: ccs', (wasm_deserialise bs t :: vs0, es0), None)>>.
+                 resolve_reduce_ctx vs0 es0.
+                 by eapply r_load_packed_success; subst; eauto.
+               + (* None *)
+                 apply <<hs, (s, (fc, lcs) :: ccs', (vs0, es0), Some AI_trap)>>.
+                 resolve_reduce_ctx vs0 es0.
+                 by eapply r_load_packed_failure; subst; eauto.
+             - destruct (load (mem_s_j) (Wasm_int.N_of_uint i32m c) off (t_length t)) as [bs|] eqn:Hload.
+               + (* Some bs *)
+                 apply <<hs, (s, (fc, lcs) :: ccs', (wasm_deserialise bs t :: vs0, es0), None)>>.
+                 resolve_reduce_ctx vs0 es0.
+                 by eapply r_load_success; subst; eauto.
+               + (* None *)
+                 apply <<hs, (s, (fc, lcs) :: ccs', (vs0, es0), Some AI_trap)>>.
+                 resolve_reduce_ctx vs0 es0.
+                 by eapply r_load_failure; subst; eauto.
+           }
+           { (* None *)
+             by admit_rsc.
+           (*
+            apply RS''_error. by eapply load_error_jth with (j := j). *)
+           }
+        * (* None *)
+          by admit_rsc.
+        (* apply RS''_error. by eapply load_error_smem_ind. *)
 
+        (*
     * (* AI_basic (BI_load t None a off) *)
       destruct ves as [|v ves'] eqn:?.
       + (* [::] *)
@@ -442,318 +657,340 @@ Proof.
               apply RS''_error. by eapply load_error_jth with (j := j).
         -- (* None *)
            apply RS''_error. by eapply load_error_smem_ind.
+*)
 
-    * (* AI_basic (BI_store t (Some tp) a off) *)
+    - (* AI_basic (BI_store t (Some tp) a off) *)
       (* TODO dedupe with the branch below by matching tp later? *)
-      destruct ves as [|v [|v' ves']] eqn:?;
-        try by (apply RS''_error; apply store_error_size).
+      get_cc ccs Hvalid.    
+      remember (fc.(FC_frame)) as f.
+      destruct vs0 as [|v [|v' vs0]].
+      1,2: by admit_rsc.
+      (*  try by (apply RS''_error; apply store_error_size). *)
       (* v :: v' :: ves' *)
-      destruct v' as [c| | |] eqn:?;
-        try by (apply RS''_error; eapply store_error_typeof => //).
+      destruct v' as [c| | |] eqn:?.
+      2,3,4: by admit_rsc.
+      (*  try by (apply RS''_error; eapply store_error_typeof => //). *)
       (* VAL_int32 c *)
       destruct (types_agree t v) eqn:?.
       + (* true *)
         destruct (smem_ind s f.(f_inst)) as [j|] eqn:?.
-        -- (* Some j *)
+        * (* Some j *)
            destruct (List.nth_error s.(s_mems) j) as [mem_s_j|] eqn:?.
-           ** (* Some mem_s_j *)
-              destruct (store_packed mem_s_j (Wasm_int.N_of_uint i32m c) off (bits v) (tp_length tp)) as [mem'|] eqn:?.
-              ++ (* Some mem' *)
-                 apply <<hs, upd_s_mem s (set_nth mem' s.(s_mems) j mem'), f, vs_to_es ves'>>'.
-                 by eapply reduce_store_packed_success with (mem_s_j := mem_s_j).
-              ++ (* None *)
-                 apply <<hs, s, f, vs_to_es ves' ++ [:: AI_trap]>>'.
-                 by eapply reduce_store_packed_failure with (j := j) (mem_s_j := mem_s_j).
-           ** (* None *)
-              apply RS''_error. by eapply store_error_jth with (j := j).
-        -- (* None *)
-           apply RS''_error. by eapply store_error_smem.
+           { (* Some mem_s_j *)
+             destruct op as [tp | ].
+              - (* Some tp*)
+                destruct (store_packed mem_s_j (Wasm_int.N_of_uint i32m c) off (bits v) (tp_length tp)) as [mem'|] eqn:?.
+                + (* Some mem' *)
+                  apply <<hs, (upd_s_mem s (set_nth mem' s.(s_mems) j mem'), (fc, lcs) :: ccs', (vs0, es0), None)>>.
+                  resolve_reduce_ctx vs0 es0.
+                  by eapply r_store_packed_success; subst; eauto.
+                + (* None *)
+                  apply <<hs, (s, (fc, lcs) :: ccs', (vs0, es0), Some AI_trap)>>.
+                  resolve_reduce_ctx vs0 es0.
+                  by eapply r_store_packed_failure; subst; eauto.
+                  (* None *)
+              - destruct (store mem_s_j (Wasm_int.N_of_uint i32m c) off (bits v) (t_length t)) as [mem'|] eqn:?.
+                + (* Some mem' *)
+                  apply <<hs, (upd_s_mem s (set_nth mem' s.(s_mems) j mem'), (fc, lcs) :: ccs', (vs0, es0), None)>>.
+                  resolve_reduce_ctx vs0 es0.
+                  by eapply r_store_success; subst; eauto.
+                + (* None *)
+                  apply <<hs, (s, (fc, lcs) :: ccs', (vs0, es0), Some AI_trap)>>.
+                  resolve_reduce_ctx vs0 es0.
+                  by eapply r_store_failure; subst; eauto.
+           }
+           { (* None *)
+             by admit_rsc.
+             (* apply RS''_error. by eapply store_error_jth with (j := j). *)
+           }
+        * (* None *)
+          by admit_rsc.
+      (*   apply RS''_error. by eapply store_error_smem. *)
       + (* false *)
-        apply RS''_error. by apply store_error_types_disagree with (v := v) (c := c) (ves' := ves').
+        by admit_rsc.
+        (*apply RS''_error. by apply store_error_types_disagree with (v := v) (c := c) (ves' := ves'). *)
 
-    * (* AI_basic (BI_store t None a off) *)
-      destruct ves as [|v [|v' ves']] eqn:?;
-        try by (apply RS''_error; apply store_error_size).
-      (* v :: v' :: ves' *)
-      destruct v' as [c| | |] eqn:?;
-        try by (apply RS''_error; eapply store_error_typeof => //).
-      (* VAL_int32 c *)
-      destruct (types_agree t v) eqn:?.
-      + (* true *)
-        destruct (smem_ind s f.(f_inst)) as [j|] eqn:?.
-        -- (* Some j *)
-           destruct (List.nth_error s.(s_mems) j) as [mem_s_j|] eqn:?.
-           ** (* Some mem_s_j *)
-              destruct (store mem_s_j (Wasm_int.N_of_uint i32m c) off (bits v) (t_length t)) as [mem'|] eqn:?.
-              ++ (* Some mem' *)
-                 apply <<hs, upd_s_mem s (set_nth mem' s.(s_mems) j mem'), f, vs_to_es ves'>>'.
-                 by eapply reduce_store_success with (mem_s_j := mem_s_j).
-              ++ (* None *)
-                 apply <<hs, s, f, vs_to_es ves' ++ [:: AI_trap]>>'.
-                 by eapply reduce_store_failure with (j := j) (mem_s_j := mem_s_j).
-           ** (* None *)
-              apply RS''_error. by eapply store_error_jth with (j := j).
-        -- (* None *)
-           apply RS''_error. by eapply store_error_smem.
-      + (* false *)
-        apply RS''_error. by apply store_error_types_disagree with (v := v) (c := c) (ves' := ves').
-
-    * (* AI_basic BI_current_memory *)
+    - (* AI_basic BI_current_memory *)
+      get_cc ccs Hvalid.    
+      remember (fc.(FC_frame)) as f.
       destruct (smem_ind s f.(f_inst)) as [j|] eqn:?.
       + (* Some j *)
         destruct (List.nth_error s.(s_mems) j) as [s_mem_s_j|] eqn:?.
-        -- (* Some j *)
-           remember (VAL_int32 (Wasm_int.int_of_Z i32m (Z.of_nat (mem_size s_mem_s_j)))) as v' eqn:?.
-           apply <<hs, s, f, vs_to_es (v' :: ves)>>'.
-           by apply reduce_current_memory with (j := j) (s_mem_s_j := s_mem_s_j).
-        -- (* None *)
-           apply RS''_error. by apply current_memory_error_jth with (j := j).
+        * (* Some j *)
+          remember (VAL_int32 (Wasm_int.int_of_Z i32m (Z.of_nat (mem_size s_mem_s_j)))) as v' eqn:?.
+          apply <<hs, (s, (fc, lcs) :: ccs', (v' :: vs0, es0), None)>>.
+          resolve_reduce_ctx vs0 es0.
+          by subst; eapply r_current_memory; eauto.
+        * (* None *)
+          by admit_rsc.
+          (* apply RS''_error. by apply current_memory_error_jth with (j := j). *)
       + (* None *)
-        apply RS''_error. by apply current_memory_error_smem => //.
+        by admit_rsc.
+        (* apply RS''_error. by apply current_memory_error_smem => //. *)
 
-    * (* AI_basic BI_grow_memory *)
-      destruct ves as [|v ves'] eqn:?;
-        try by (apply RS''_error; apply grow_memory_error_0).
+    - (* AI_basic BI_grow_memory *)
+      get_cc ccs Hvalid.    
+      remember (fc.(FC_frame)) as f.
+      destruct vs0 as [|v vs0]; first by admit_rsc.
+      (*  try by (apply RS''_error; apply grow_memory_error_0). *)
       (* v :: ves' *)
-      destruct v as [c| | |] eqn:?;
-        try by (apply RS''_error; by eapply grow_memory_error_typeof => //).
+      destruct v as [c| | |] eqn:?.
+      2,3,4: by admit_rsc.
+      (*  try by (apply RS''_error; by eapply grow_memory_error_typeof => //). *)
       (* VAL_int32 c *)
       destruct (smem_ind s f.(f_inst)) as [j|] eqn:?.
       + (* Some j *)
         destruct (List.nth_error s.(s_mems) j) as [s_mem_s_j|] eqn:Heqsmem.
-        -- (* Some s_mem_s_j *)
+        * (* Some s_mem_s_j *)
            remember (mem_grow s_mem_s_j (Wasm_int.N_of_uint i32m c)) as mem'.
            destruct mem' as [mem''|].
-           ** (* Some mem'' *)
+           -- (* Some mem'' *)
               remember (VAL_int32 (Wasm_int.int_of_Z i32m (Z.of_nat (mem_size s_mem_s_j)))) as v'.
               remember (upd_s_mem s (set_nth mem'' s.(s_mems) j mem'')) as s'.
-              apply <<hs, s', f, (vs_to_es (v' :: ves'))>>'.
-              by eapply reduce_grow_memory with (j := j) (s_mem_s_j := s_mem_s_j) (mem'' := mem'') => //.
-           ** (* None *)
-              apply <<hs, s, f, vs_to_es (VAL_int32 int32_minus_one :: ves')>>'.
-              by eapply reduce_grow_memory_failure with (j := j) (s_mem_s_j := s_mem_s_j).
-        -- (* None *)
-           apply RS''_error. by eapply grow_memory_error_jth with (j := j).
+              apply <<hs, (s', (fc, lcs) :: ccs', (v' :: vs0, es0), None)>>.
+              resolve_reduce_ctx vs0 es0.
+              by subst; eapply r_grow_memory_success; eauto.
+           -- (* None *)
+              apply <<hs, (s, (fc, lcs) :: ccs', (VAL_int32 int32_minus_one :: vs0, es0), None)>>.
+              resolve_reduce_ctx vs0 es0.
+              by subst; eapply r_grow_memory_failure; eauto.
+        * (* None *)
+          by admit_rsc.
+          (* apply RS''_error. by eapply grow_memory_error_jth with (j := j). *)
       + (* None *)
-        apply RS''_error. by eapply grow_memory_error_smem => //.
+        by admit_rsc.
+        (* apply RS''_error. by eapply grow_memory_error_smem => //. *)
 
-    * (* AI_basic (BI_const _) *)
-      by exfalso.
+    - (* AI_basic (BI_const _) *)
+      unfold valid_cfg_ctx, valid_ccs, valid_split in Hvalid => /=.
+      by inversion Hvalid.
 
-    * (* AI_basic (BI_unop t op) *)
-      destruct ves as [|v ves'].
+    - (* AI_basic (BI_unop t op) *)
+      destruct vs0 as [|v vs0].
       + (* [::] *)
-        apply RS''_error. by apply unop_error.
+        by admit_rsc.
+        (* apply RS''_error. by apply unop_error. *)
       + (* v :: ves' *)
-        apply <<hs, s, f, vs_to_es (app_unop op v :: ves')>>'.
-        by apply reduce_unop.
+        apply <<hs, (s, ccs, (app_unop op v :: vs0, es0), None)>>.
+        resolve_reduce_ctx vs0 es0.
+        by apply r_simple, rs_unop.
 
-    * (* AI_basic (BI_binop t op) *)
-      destruct ves as [|v2 [|v1 ves']];
-        try by (apply RS''_error; apply binop_error_size).
+    - (* AI_basic (BI_binop t op) *)
+      destruct vs0 as [|v2 [|v1 vs0]].
+      1,2: by admit_rsc.
+      (*  try by (apply RS''_error; apply binop_error_size). *)
       (* [:: v2, v1 & ves'] *)
       destruct (app_binop op v1 v2) as [v|] eqn:?.
       + (* Some v *)
-        apply <<hs, s, f, vs_to_es (v :: ves')>>'.
-        by apply reduce_binop.
+        apply <<hs, (s, ccs, (v :: vs0, es0), None)>>.
+        resolve_reduce_ctx vs0 es0.
+        by apply r_simple, rs_binop_success.
       + (* None *)
-        apply <<hs, s, f, (vs_to_es ves') ++ [:: AI_trap]>>'.
-        by apply reduce_binop_trap.
+        apply <<hs, (s, ccs, (vs0, es0), Some AI_trap)>>.
+        resolve_reduce_ctx vs0 es0.
+        by apply r_simple, rs_binop_failure.
 
-    * (* AI_basic (BI_testop T_i32 testop) *)
-      destruct ves as [|[c| | |] ves'] eqn:?;
-        try by (apply RS''_error; by eapply testop_i32_error => //).
+    - (* AI_basic (BI_testop t testop) *)
+      destruct vs0 as [| v vs0].
+      (*  try by (apply RS''_error; by eapply testop_i32_error => //). *)
       + (* [::] *)
-        apply RS''_error. by apply testop_error_0.
+        by admit_rsc.
+        (* apply RS''_error. by apply testop_error_0. *)
       + (* VAL_int32 c :: ves' *)
-        apply <<hs, s, f, vs_to_es (VAL_int32 (wasm_bool (@app_testop_i i32t testop c)) :: ves')>>'.
-        by apply reduce_testop_i32.
+        destruct t as [| | |].
+        3,4: by admit_rsc.
+        (* i32 *)
+        * destruct v as [c| | |].
+          2,3,4: by admit_rsc.
+          apply <<hs, (s, ccs, (VAL_int32 (wasm_bool (@app_testop_i i32t testop c)) :: vs0, es0), None)>>.
+          resolve_reduce_ctx vs0 es0.
+          by apply r_simple, rs_testop_i32.
+        (* i64 *)
+        * destruct v as [|c | |].
+          1,3,4: by admit_rsc.
+          apply <<hs, (s, ccs, (VAL_int32 (wasm_bool (@app_testop_i i64t testop c)) :: vs0, es0), None)>>.
+          resolve_reduce_ctx vs0 es0.
+          by apply r_simple, rs_testop_i64.
 
-    * (* AI_basic (BI_testop T_i64 testop) *)
-      (* TODO un-nest this destruct? could make the 'try by' clearer *)
-      destruct ves as [|v ves'].
-      + (* [::] *)
-        apply RS''_error. by apply testop_error_0.
-      + (* v :: ves' *)
-        destruct v as [|c| |];
-          try by (apply RS''_error; by eapply testop_i64_error => //).
-        (* VAL_int64 c *)
-        apply <<hs, s, f, vs_to_es (VAL_int32 (wasm_bool (@app_testop_i i64t testop c)) :: ves')>>'.
-        by eapply reduce_testop_i64.
-
-    * (* AI_basic (BI_testop T_f32 testop) *)
-      apply RS''_error. by apply testop_f32_error.
-
-    * (* AI_basic (BI_testop T_f64 testop) *)
-      apply RS''_error. by apply testop_f64_error.
-
-    * (* AI_basic (BI_relop t op) *)
-      destruct ves as [|v2 [|v1 ves']];
-          try by (apply RS''_error; apply relop_error_size).
+    - (* AI_basic (BI_relop t op) *)
+      destruct vs0 as [|v2 [|v1 vs0]].
+      1,2: by admit_rsc.
+      (*    try by (apply RS''_error; apply relop_error_size). *)
       (* [:: v2, v1 & ves'] *)
-      apply <<hs, s, f, vs_to_es (VAL_int32 (wasm_bool (app_relop op v1 v2)) :: ves')>>'.
-      by apply reduce_relop.
+      apply <<hs, (s, ccs, (VAL_int32 (wasm_bool (@app_relop op v1 v2)) :: vs0, es0), None)>>.
+      resolve_reduce_ctx vs0 es0.
+      by apply r_simple, rs_relop.
 
-    * (* AI_basic (BI_cvtop t2 CVO_convert t1 sx) *)
-      destruct ves as [|v ves'];
-        try by (apply RS''_error; apply cvtop_error_0).
+    - (* AI_basic (BI_cvtop t2 CVO_convert t1 sx) *)
+      destruct vs0 as [|v vs0]; first by admit_rsc.
+       (* try by (apply RS''_error; apply cvtop_error_0). *)
       (* v :: ves' *)
       destruct (types_agree t1 v) eqn:Ht1.
       + (* true *)
-        destruct (cvt t2 sx v) as [v'|] eqn:Heqv'.
-        -- (* Some v' *)
-           apply <<hs, s, f, vs_to_es (v' :: ves')>>'.
-           by apply reduce_cvtop_success.
-        -- (* None *)
-           apply <<hs, s, f, vs_to_es ves' ++ [::AI_trap]>>'.
-           by apply reduce_cvtop_trap.
+        destruct cvtop.
+        (* convert *)
+        * destruct (cvt t2 sx v) as [v'|] eqn:Heqv'.
+          { (* Some v' *)
+            apply <<hs, (s, ccs, (v' :: vs0, es0), None)>>.
+            resolve_reduce_ctx vs0 es0.
+            by apply r_simple, rs_convert_success.
+          }
+          { (* None *)
+            apply <<hs, (s, ccs, (vs0, es0), Some AI_trap)>>.
+            resolve_reduce_ctx vs0 es0.
+            by apply r_simple, rs_convert_failure.
+          }
+        (* Reinterpret *)
+        * destruct sx eqn:Heqsx.
+          { (* Some _ *)
+            (* apply RS''_error. by eapply cvtop_error_reinterpret_sx. *)
+            by admit_rsc.
+          }
+          { (* None *)
+            apply <<hs, (s, ccs, ((wasm_deserialise (bits v) t2) :: vs0, es0), None)>>.
+            resolve_reduce_ctx vs0 es0.
+            by apply r_simple, rs_reinterpret.
+          }
       + (* false *)
-        apply RS''_error. by eapply cvtop_error_types_disagree.
+        by admit_rsc.
+        (* apply RS''_error. by eapply cvtop_error_types_disagree. *)
 
-    * (* AI_basic (BI_cvtop t2 CVO_reinterpret t1 sx) *)
-      destruct ves as [|v ves'];
-        try by (apply RS''_error; apply cvtop_error_0).
-      destruct (types_agree t1 v) eqn:?.
-      + (* true *)
-        destruct sx eqn:Heqsx.
-        -- (* Some _ *)
-           apply RS''_error. by eapply cvtop_error_reinterpret_sx.
-        -- (* None *)
-           apply <<hs, s, f, (vs_to_es (wasm_deserialise (bits v) t2 :: ves'))>>'.
-           by apply reduce_reinterpret.
-      + (* false *)
-        apply RS''_error. by eapply cvtop_error_types_disagree.
+    - (* AI_trap *)
+      get_cc ccs Hvalid.
+      destruct ((vs0 == nil) && (es0 == nil)) eqn:Hscnil; move/andP in Hscnil.
+      + destruct Hscnil as [Heq1 Heq2]; move/eqP in Heq1; move/eqP in Heq2; subst.
+        destruct lcs as [ | lc lcs'].
+        * destruct fc as [lvs ? ? les].
+          apply <<hs, (s, ccs', (lvs, les), Some AI_trap)>> => /=.
+          resolve_reduce_ctx lvs les.
+          by apply r_simple, rs_local_trap.
+        * destruct lc as [lvs ? ? les].
+          apply <<hs, (s, (fc, lcs') :: ccs', (lvs, les), Some AI_trap)>>.
+          unfold reduce_ctx.
+          apply reduce_focus_ctx => //=.
+          apply list_label_ctx_eval.(ctx_reduce) => //=.
+          unfold label_ctx_fill => /=.
+          resolve_reduce_ctx lvs les.
+          by apply r_simple, rs_label_trap.
+      + apply <<hs, (s, (fc, lcs) :: ccs', (nil, nil), Some AI_trap)>>.
+        resolve_reduce_ctx lvs les.
+        apply r_simple.
+        apply rs_trap with (lh := LH_base (rev vs0) es0) => //.
+        move => Hcontra; apply Hscnil.
+        specialize (f_equal size Hcontra) as Hsize; rewrite size_cat v_to_e_size size_rev in Hsize.
+        simpl in Hsize.
+        clear - Hsize.
+        assert (H: size vs0 = 0); first (by lias); destruct vs0 => //; clear H.
+        assert (H: size es0 = 0); first (by lias); by destruct es0.
 
-    * (* AI_trap *)
-      by exfalso.
-
-    * (* AI_invoke a *)
+    - (* AI_invoke a *)
+      get_cc ccs Hvalid.    
       destruct (List.nth_error s.(s_funcs) a) as [cl|] eqn:?.
       + (* Some cl *)
         destruct cl as [i [t1s t2s] ts es | [t1s t2s] cl'] eqn:?.
-        -- (* FC_func_native i (Tf t1s t2s) ts es *)
+        * (* FC_func_native i (Tf t1s t2s) ts es *)
            remember (length t1s) as n eqn:?.
            remember (length t2s) as m eqn:?.
-           destruct (length ves >= n) eqn:?.
-           ** (* true *)
-              destruct (split_n ves n) as [ves' ves''] eqn:?.
-              remember (n_zeros ts) as zs eqn:?.
-              apply <<hs, s, f, vs_to_es ves'' ++ [::
-                AI_local
-                m
-                (Build_frame (rev ves' ++ zs) i)
-                [::AI_basic (BI_block (Tf [::] t2s) es)]
-              ]>>'.
-              by eapply reduce_invoke_native with (n := n) (ts := ts) (t1s := t1s).
-           ** (* false *)
-              apply RS''_error.
+           destruct (length vs0 >= n) eqn:Hlen.
+           -- (* true *)
+             destruct (split_n vs0 n) as [vs' vs''] eqn:Hsplit.
+             remember (n_zeros ts) as zs eqn:?.
+             apply <<hs, (s, (Build_frame_ctx vs'' m (Build_frame (rev vs' ++ zs) i) es0, nil) :: (fc, lcs) :: ccs', (nil, nil), Some (AI_basic (BI_block (Tf [::] t2s) es)))>> => /=.
+             red_ctx_simpl => //.
+             eapply r_label with (lh := LH_base (rev (FC_val fc)) (FC_post fc)) => /=; infer_hole.
+             apply r_local.
+             red_ctx_simpl => //=.
+             rewrite split_n_is_take_drop in Hsplit.
+             injection Hsplit as ??.
+             eapply r_label with (lh := LH_base (rev vs'') es0) => /=; subst; infer_hole.
+             2: { instantiate (1 := (v_to_e_list (rev (take (length t1s) vs0)) ++ [::AI_invoke a])).
+                  by rewrite catA catA v_to_e_cat -rev_cat cat_take_drop -catA.
+             }
+             eapply r_invoke_native; eauto.
+             repeat rewrite length_is_size.
+             repeat rewrite length_is_size in Hlen.
+             by rewrite size_rev size_takel => //.
+           -- (* false *)
+             by admit_rsc.
+             (* apply RS''_error.
               by eapply invoke_func_native_error_n with
-                (n := n) (t1s := t1s) (t2s := t2s) (i := i) (ts := ts) (es := es).
-        -- (* FC_func_host (Tf t1s t2s) cl' *)
+                (n := n) (t1s := t1s) (t2s := t2s) (i := i) (ts := ts) (es := es). *)
+        * (* FC_func_host (Tf t1s t2s) cl' *)
            remember (length t1s) as n eqn:?.
            remember (length t2s) as m eqn:?.
-           destruct (length ves >= n) eqn:?.
-           ** (* true *)
-              destruct (split_n ves n) as [ves' ves''] eqn:?.
-              destruct (host_application_impl hs s (Tf t1s t2s) cl' (rev ves')) as [hs' [[s' rves]|]] eqn:?.
+           destruct (length vs0 >= n) eqn:Hlen.
+           -- (* true *)
+              destruct (split_n vs0 n) as [vs' vs''] eqn: Hsplit.
+              destruct (host_application_impl hs s (Tf t1s t2s) cl' (rev vs')) as [hs' [[s' rves]|]] eqn:?.
               ++ (* (hs', Some (s', rves)) *)
-                 apply <<hs', s', f, vs_to_es ves'' ++ (result_to_stack rves)>>'.
-                 by eapply reduce_invoke_host_success with
-                   (n := n) (t1s := t1s) (t2s := t2s) (cl' := cl') (ves' := ves').
+                destruct rves as [rvs | ].
+                ** apply <<hs', (s', (fc, lcs) :: ccs', (rev rvs ++ vs'', es0), None)>> => /=.
+                   red_ctx_simpl => //.
+                   eapply r_label with (lh := LH_base (rev (FC_val fc)) (FC_post fc)) => /=; infer_hole.
+                   apply r_local.
+                   red_ctx_simpl => //=.
+                   rewrite split_n_is_take_drop in Hsplit.
+                   injection Hsplit as ??.
+                   eapply r_label with (lh := LH_base (rev vs'') es0) => /=; subst; infer_hole.
+                   2: { instantiate (1 := (v_to_e_list (rev (take (length t1s) vs0)) ++ [::AI_invoke a])).
+                        by rewrite catA catA v_to_e_cat -rev_cat cat_take_drop -catA.
+                   }
+                   rewrite revK.
+                   unfold fmask0 => /=.
+                   fold (result_to_stack (result_values rvs)).
+                   eapply r_invoke_host_success; eauto.
+                   repeat rewrite length_is_size.
+                   by rewrite size_rev size_takel => //.
+                ** apply <<hs', (s', (fc, lcs) :: ccs', (vs'', es0), Some AI_trap)>> => /=.
+                   red_ctx_simpl => //.
+                   eapply r_label with (lh := LH_base (rev (FC_val fc)) (FC_post fc)) => /=; infer_hole.
+                   apply r_local.
+                   red_ctx_simpl => //=.
+                   rewrite split_n_is_take_drop in Hsplit.
+                   injection Hsplit as ??.
+                   eapply r_label with (lh := LH_base (rev vs'') es0) => /=; subst; infer_hole.
+                   2: { instantiate (1 := (v_to_e_list (rev (take (length t1s) vs0)) ++ [::AI_invoke a])).
+                        by rewrite catA catA v_to_e_cat -rev_cat cat_take_drop -catA.
+                   }
+                   unfold fmask0 => /=.
+                   fold (result_to_stack result_trap).
+                   eapply r_invoke_host_success; eauto.
+                   repeat rewrite length_is_size.
+                   by rewrite size_rev size_takel => //.
               ++ (* (hs', None) *)
-                 apply <<hs', s, f, vs_to_es ves ++ [::AI_invoke a]>>'.
-                 by eapply reduce_invoke_host_diverge with
-                   (n := n) (t1s := t1s) (t2s := t2s) (cl' := cl') (ves' := ves') (ves'' := ves'') => //.
-           ** (* false *)
+                   apply <<hs', (s, (fc, lcs) :: ccs', (vs'', es0), Some AI_trap)>> => /=.
+                   red_ctx_simpl => //.
+                   eapply r_label with (lh := LH_base (rev (FC_val fc)) (FC_post fc)) => /=; infer_hole.
+                   apply r_local.
+                   red_ctx_simpl => //=.
+                   rewrite split_n_is_take_drop in Hsplit.
+                   injection Hsplit as ??.
+                   eapply r_label with (lh := LH_base (rev vs'') es0) => /=; subst; infer_hole.
+                   2: { instantiate (1 := (v_to_e_list (rev (take (length t1s) vs0)) ++ [::AI_invoke a])).
+                        by rewrite catA catA v_to_e_cat -rev_cat cat_take_drop -catA.
+                   }
+                   unfold fmask0 => /=.
+                   eapply r_invoke_host_diverge; eauto.
+                   repeat rewrite length_is_size.
+                   by rewrite size_rev size_takel => //.
+           -- (* false *)
+             by admit_rsc.
+             (*
               apply RS''_error.
               by eapply invoke_func_host_error_n with
                 (n := n) (t1s := t1s) (t2s := t2s) (cl' := cl').
+              *)
       + (* None *)
-        apply RS''_error. by apply invoke_host_error_ath.
+        by admit_rsc.
+        (* apply RS''_error. by apply invoke_host_error_ath. *)
 
-    * (* AI_label ln les es *)
-      destruct (es_is_trap es) eqn:?.
-      + (* true *)
-        apply <<hs, s, f, vs_to_es ves ++ [::AI_trap]>>'.
-        by apply reduce_label_trap.
-      + (* false *)
-        destruct (const_list es) eqn:?.
-        -- (* true *)
-           apply <<hs, s, f, vs_to_es ves ++ es>>'.
-           by apply reduce_label_const.
-        -- (* false *)
-          assert (run_step_measure es < S (run_one_step_measure (AI_label ln les es)))%coq_nat as Hmeasure.
-          { simpl. by rewrite run_step_measure_eq; lias. }
-          specialize (run_step_aux hs s f es Hmeasure).
-          destruct run_step_aux as
-             [ Hv | Herr | n bvs H | rvs H | hs' s' f' es'] eqn:?.
-           ** (* RS'_value hs s f Hv *)
-              exfalso. by apply const_trap_contradiction with (es := es).
-           ** (* RS'_error hs Herr *)
-              apply RS''_error.
-              by apply label_error_rec.
-           ** (* RS'_break hs s f es n bvs *)
-              destruct n as [|n].
-              ++ (* 0 *)
-                 destruct (length bvs >= ln) eqn:?.
-                 --- (* true *)
-                     apply <<hs, s, f, vs_to_es ((take ln bvs) ++ ves) ++ les>>'.
-                     by apply reduce_label_break_rec.
-                 --- (* false *)
-                     apply RS''_error.
-                     by apply label_error_break_rec with (bvs := bvs).
-              ++ (* n.+1 *)
-                 apply break(n, bvs).
-                 by apply label_break_rec.
-           ** (* RS'_return hs s f es rvs H *)
-              apply RS''_return with (rvs := rvs).
-              (* TODO move into a lemma? *)
-              right. destruct H as [i [lh H]].
-              by exists ln, les, es, i, lh => //.
-           ** (* RS'_normal hs s f es hs' s' f' es' *)
-              apply <<hs', s', f', vs_to_es ves ++ [:: AI_label ln les es']>>'.
-              by apply reduce_label_rec.
+        
+    - (* AI_label ln les es *)
+      by inversion Hvalid.
 
     * (* AI_local ln lf es *)
-      destruct (es_is_trap es) eqn:?.
-      + (* true *)
-        apply <<hs, s, f, vs_to_es ves ++ [::AI_trap]>>'.
-        by apply reduce_local_trap.
-      + (* false *)
-        destruct (const_list es) eqn:?.
-        -- (* true *)
-           destruct (length es == ln) eqn:?.
-           ** (* true *)
-              apply <<hs, s, f, vs_to_es ves ++ es>>'.
-              by apply reduce_local_const.
-           ** (* false *)
-              apply RS''_error.
-              by apply local_error_const_len.
-        -- (* false *)
-           assert (run_step_measure es < S (run_one_step_measure (AI_local ln lf es)))%coq_nat as Hmeasure.
-           { simpl. by rewrite run_step_measure_eq; lias. }
-           specialize (run_step_aux hs s lf es Hmeasure).
-           destruct run_step_aux as
-             [ Hv | Herr | n bvs | rvs H | hs' s' f' es'] eqn:?; clear Hmeasure.
-           ** (* RS'_value hs s f Hv *)
-              exfalso. by apply const_trap_contradiction with (es := es).
-           ** (* RS'_error hs Herr *)
-              apply RS''_error.
-              by apply local_error_rec.
-           ** (* RS'_break hs s f es n bvs *)
-              apply RS''_error.
-              by apply local_error_break_rec with (n := n) (bvs := bvs).
-           ** (* RS'_return hs s f es rvs H *)
-              destruct (length rvs >= ln) eqn:?.
-              ++ (* true *)
-                 apply <<hs, s, f, vs_to_es (take ln rvs ++ ves)>>'.
-                 by apply reduce_local_return_rec.
-              ++ (* false *)
-                 apply RS''_error.
-                 apply local_return_error with (rvs := rvs) => //.
-           ** (* RS'_normal hs s f es hs' s' f' es' *)
-              apply <<hs', s', f, vs_to_es ves ++ [:: AI_local ln f' es']>>'.
-              by apply reduce_local_rec.
+      by inversion Hvalid.
+  }
 Defined.
 
 End Host.
